wip

Foundation/Modal/Neighborhood/Completeness.lean
@@ -86,41 +86,65 @@ open Formula.Neighborhood
 open MaximalConsistentSet
 
 variable {S} [Entailment (Formula ℕ) S]
-variable {𝓢 : S} [Entailment.Cl 𝓢] [Entailment.Consistent 𝓢]
+variable {𝓢 : S} -- [Entailment.Cl 𝓢] [Entailment.Consistent 𝓢]
 variable {φ ψ ξ : Formula ℕ}
 
-structure CanonicalBox (𝓢 : S) where
-  box : Set (MaximalConsistentSet 𝓢) → Set (MaximalConsistentSet 𝓢)
-  canonicity : ∀ φ, box (proofset 𝓢 φ) = proofset 𝓢 (□φ)
+class Frame.IsCanonical (F : Frame) (𝓢 : S) : Prop where
+  eq_world : F.World = MaximalConsistentSet 𝓢 := by rfl
+  box_proofset : ∀ φ, F.box (eq_world ▸ (proofset 𝓢 φ)) = eq_world ▸ (proofset 𝓢 (□φ))
+
+namespace Frame.IsCanonical
+
+variable {F : Frame} [canonical : F.IsCanonical 𝓢]
+
+@[simp]
+lemma eq_empty : (canonical.eq_world ▸ (∅ : Set (MaximalConsistentSet 𝓢))) = ∅ := by
+  have := canonical.eq_world;
+  grind;
+
+@[simp]
+lemma eq_union {X Y : Set (MaximalConsistentSet 𝓢)} : (canonical.eq_world ▸ (X ∪ Y)) = ((canonical.eq_world ▸ X) ∪ (canonical.eq_world ▸ Y)) := by
+  have := canonical.eq_world;
+  grind;
+
+@[simp]
+lemma eq_comp {X : Set (MaximalConsistentSet 𝓢)} : (canonical.eq_world ▸ Xᶜ) = (canonical.eq_world ▸ X)ᶜ := by
+  haveI := canonical.eq_world;
+  grind;
+
+@[simp]
+lemma iff_mem {Γ : MaximalConsistentSet 𝓢} {X : Set _} : Γ ∈ X ↔ (canonical.eq_world ▸ Γ) ∈ (canonical.eq_world ▸ X) := by
+  have := canonical.eq_world;
+  grind;
+
+end Frame.IsCanonical
 
 
-variable {𝓑 : CanonicalBox 𝓢}
+def canonicalModel (F : Frame) (𝓢 : S) [canonical : F.IsCanonical 𝓢] : Model where
+  toFrame := F
+  Val a := canonical.eq_world ▸ proofset 𝓢 (.atom a)
 
-namespace CanonicalBox
+namespace canonicalModel
 
-instance : CoeFun (CanonicalBox 𝓢) (fun _ => Set (MaximalConsistentSet 𝓢) → Set (MaximalConsistentSet 𝓢)) := ⟨CanonicalBox.box⟩
+variable {F : Frame} [canonical : F.IsCanonical 𝓢]
 
-protected def frame (𝓑 : CanonicalBox 𝓢) : Frame := Frame.mk_ℬ (MaximalConsistentSet 𝓢) 𝓑
+@[simp] lemma eq_model_box : (canonicalModel F 𝓢).box = F.box := by tauto;
 
-protected def model (𝓑 : CanonicalBox 𝓢) : Model where
-  toFrame := 𝓑.frame
-  Val a := proofset 𝓢 (.atom a)
+end canonicalModel
 
-@[simp] lemma eq_model_box : 𝓑.model.box = 𝓑 := by tauto;
+variable [Entailment.Cl 𝓢]
+         {F : Frame} [canonical : F.IsCanonical 𝓢]
 
-end CanonicalBox
-
-
-lemma truthlemma : ↑(proofset 𝓢 φ) = (𝓑.model.truthset φ) := by
+lemma truthlemma : canonical.eq_world ▸ (proofset 𝓢 φ) = ((canonicalModel F 𝓢).truthset φ) := by
   induction φ with
-  | hatom => simp [CanonicalBox.model]
-  | hfalsum => simp [CanonicalBox.model]
-  | himp φ ψ ihφ ihψ =>
-    simp_all [MaximalConsistentSet.proofset.eq_imp, ←ihφ, ←ihψ];
+  | hatom => simp [canonicalModel]
+  | hfalsum => simp [canonicalModel];
+  | himp φ ψ ihφ ihψ => simp_all [MaximalConsistentSet.proofset.eq_imp, ←ihφ, ←ihψ];
   | hbox φ ihφ =>
-    rw [Model.truthset.eq_box, ←ihφ, CanonicalBox.eq_model_box, (@𝓑.canonicity φ)];
+    rw [Model.truthset.eq_box, ←ihφ, ←(canonical.box_proofset φ)];
+    rfl;
 
-lemma complete_of_canonical_frame (C : FrameClass) (𝓑 : CanonicalBox 𝓢) (hC : 𝓑.frame ∈ C)
+lemma complete_of_canonical_frame (C : FrameClass) (F : Frame) [canonical : F.IsCanonical 𝓢] (hC : F ∈ C)
   : LO.Complete 𝓢 C := by
   constructor;
   intro φ;
@@ -129,47 +153,52 @@ lemma complete_of_canonical_frame (C : FrameClass) (𝓑 : CanonicalBox 𝓢) (h
   have := FormulaSet.unprovable_iff_singleton_neg_consistent.mpr hφ;
   obtain ⟨Γ, hΓ⟩ := lindenbaum this;
   apply not_validOnFrameClass_of_exists_model_world;
-  use 𝓑.model, Γ;
+  use (canonicalModel F 𝓢), (canonical.eq_world ▸ Γ);
   constructor;
   . assumption;
   . simp only [Semantics.Realize, Satisfies, ←truthlemma];
-    suffices Γ ∈ (proofset 𝓢 (∼φ)) by simpa;
+    suffices Γ ∈ (proofset 𝓢 (∼φ)) by
+      apply canonical.iff_mem.not.mp;
+      simpa using this;
     apply hΓ;
     tauto;
 
 
 
+
 open Classical in
-protected abbrev CanonicalBox.minimal (𝓢 : S) [Entailment.E 𝓢] : CanonicalBox 𝓢 where
-  box Γ := if h : ∃ φ, Γ = (proofset 𝓢 φ) then (proofset 𝓢 (□(h.choose))) else ∅
-  canonicity := by
+abbrev minimalCanonicalFrame (𝓢 : S) [Entailment.E 𝓢] [Entailment.Consistent 𝓢] : Frame := Frame.mk_ℬ
+  (MaximalConsistentSet 𝓢)
+  (λ X => if h : ∃ φ, X = (proofset 𝓢 φ) then (proofset 𝓢 (□(h.choose))) else ∅)
+
+namespace minimalCanonicalFrame
+
+variable {𝓢 : S} [Entailment.E 𝓢] [Entailment.Consistent 𝓢]
+
+instance : (minimalCanonicalFrame 𝓢).IsCanonical 𝓢 where
+  box_proofset := by
     intro φ;
+    dsimp [minimalCanonicalFrame, Frame.mk_ℬ, Frame.box];
     split;
     . rename_i h;
       apply proofset.eq_boxed_of_eq;
       apply h.choose_spec.symm;
     . tauto;
 
-namespace CanonicalBox.minimal
-
-variable {𝓢 : S} [Entailment.E 𝓢] [Consistent 𝓢]
-
-lemma exists_box (X) (Γ : (CanonicalBox.minimal 𝓢).model.World) (hΓ : Γ ∈ Frame.box _ X)
+lemma exists_box (X) (Γ : (minimalCanonicalFrame 𝓢).World) (hΓ : Γ ∈ Frame.box _ X)
   : ∃ φ, X = proofset 𝓢 φ ∧ Frame.box _ X = proofset 𝓢 (□φ)
   := by
-    simp only [
-      CanonicalBox.minimal, CanonicalBox.model, CanonicalBox.frame, Frame.mk_ℬ, Frame.box,
-      Set.mem_setOf_eq, Set.setOf_mem_eq
-    ] at hΓ;
+    simp [Frame.mk_ℬ, Frame.box] at hΓ;
     split at hΓ;
     . rename_i h;
       obtain ⟨φ, hφ⟩ := h;
       use φ;
       constructor;
       . assumption;
-      . convert CanonicalBox.minimal 𝓢 |>.canonicity φ;
+      . convert Frame.IsCanonical.box_proofset (F := minimalCanonicalFrame 𝓢) (𝓢 := 𝓢) φ;
     . contradiction;
 
+/-
 lemma exists_dia (X) (Γ : (CanonicalBox.minimal 𝓢).model.World) (hΓ : Γ ∈ Frame.box _ X)
   : ∃ φ, X = proofset 𝓢 φ ∧ Frame.dia _ X = proofset 𝓢 (◇φ)
   := by
@@ -205,8 +234,9 @@ lemma exists_dia (X) (Γ : (CanonicalBox.minimal 𝓢).model.World) (hΓ : Γ �
           rw [←h₂.choose_spec, hφ];
           simp;
         . tauto;
+-/
 
-end CanonicalBox.minimal
+end minimalCanonicalFrame
 
 
 end Neighborhood
